Definitions for G-systems are done, testing them now

HOL/ProofTheoryScript.sml
@@ -44,7 +44,7 @@ val (Nm_rules, Nm_induct, Nm_cases) = Hol_reln `
 /\ (!A B D. Nm D B ==> Nm D (A Or B)) (* Or Intro left *)
 /\ (!A B C D1 D2 D3 D4. (Nm D1 (A Or B)) /\
 (Nm D2 C) /\ (Nm D3 C) /\     (* T&S say A and B need not actually be in D2 and D3 respectively *)
-(D4 = ((D1 UNION D2 UNION D3) DIFF {A;B})) ==> Nm D4 C)`;                         (* Or Elim *)
+(D4 = ((D1 UNION D2 UNION D3) DIFF {A;B})) ==> Nm D4 C)`; (* Or Elim *)
 
 (** Natural Deduction for intuitionistic logic **)
 (* Ni is the 'deduciblility' relation for this system *)
@@ -77,8 +77,9 @@ val (Nc_rules, Nc_induct, Nc_cases) = Hol_reln `
 (Nc D2 C) /\ (Nc D3 C) /\
 (D4 = ((D1 UNION D2 UNION D3) DIFF {A;B})) ==> Nc D4 C) (* Or Elim *)
 /\ (!A D. (Nc D Bot) ==> (Nc D A)) (* Intuitionistic Absurdity Rule *)
-/\ (!A D1 D2. (Nc D1 (Not A)) /\ (D2 = (D1 DIFF {Not A})) ==> Nc D2 A) (* Classical absurdidty rule *)
-`;
+/\ (!A D1 D2. (Nc D1 (Not A)) /\ (D2 = (D1 DIFF {Not A}))
+   ==> Nc D2 A)`; (* Classical absurdidty rule *)
+
 
 val NmThm = Define `NmThm A = Nm EMPTY A`;
 val NiThm = Define `NiThm A = Ni EMPTY A`;
@@ -112,37 +113,82 @@ rw[NiThm]);
 (* (* Stuck *) *)
 (* ); *)
 
-(* Need to make all the D's SING or EMPTY *)
+(** Sequent Calculus (Gentzen System) for minimal logic **)
+(* Gm is the 'deduciblility' relation for this system *)
+(* A, B and C are used to represent formulae *)
+(* S is used to represent the multiset of the Antecedent Context *)
+(* The consequent is always a single formula in the minimal logic *)
+
+val (Gm_rules, Gm_induct, Gm_cases) = Hol_reln `
+(!A:'a formula. Gm {|A|} A)            (* Ax *)
+/\ (!A S C. Gm S D ==> Gm (BAG_INSERT A S) C) (* Left Weakening *)
+/\ (!A S C. (Gm S C) /\ (S A >= 2)
+   ==> Gm (S - {|A|}) C) (* Left Contraction *)
+/\ (!A B S C. (Gm (BAG_INSERT A S) C)
+   ==> (Gm (BAG_INSERT (A And B) S) C)) (* Left And 1 *)
+/\ (!A B S C. (Gm (BAG_INSERT B S) C)
+   ==> (Gm (BAG_INSERT (A And B) S) C)) (* Left And 2 *)
+/\ (!A B S. (Gm S A) /\ (Gm S B)
+   ==> (Gm S (A And B))) (* Right And *)
+/\ (!A B S C. (Gm (BAG_INSERT A S) C)
+    /\ (Gm (BAG_INSERT B S) C)
+   ==> (Gm (BAG_INSERT (A Or B) S) C)) (* Left Or *)
+/\ (!A B S. (Gm S A)
+   ==> (Gm S (A Or B))) (* Right Or 1 *)
+/\ (!A B S. (Gm S B)
+   ==> (Gm S (A Or B))) (* Right Or 2 *)
+/\ (!A B S C. (Gm S A) /\ (Gm (BAG_INSERT B S) C)
+   ==> (Gm (BAG_INSERT (A Imp B) S) C)) (* Left Imp *)
+/\ (!A B S. (Gm (BAG_INSERT A S) B)
+   ==> (Gm S (A Imp B)))`; (* Right Imp *)
+
+val GmThm = Define `GmThm A = Gm EMPTY_BAG A`;
+
+val Gm_example1 = Q.prove(`GmThm ((A And B) Imp (B And A))`, rw[GmThm,Gm_rules]);
+
+val Gm_example2 = Q.prove(`GmThm ((A Imp (A Imp B)) Imp (A Imp B))`,
+rw[GmThm] >>
+
+);
+
+(** Sequent Calculus (Gentzen System) for intuitionistic logic **)
+(* Gi is the 'deduciblility' relation for this system *)
+(* S and D are used to represent the multiset of Antecedent and Consequent Contexts *)
+(* The Consequent has at most one formula for intuitionistic logic *)
+               
 val (Gi_rules, Gi_induct, Gi_cases) = Hol_reln `
 (!A:'a formula. Gc {|A|} {|A|})            (* Ax *)
-/\ (Gc {|Bot|} {||})            (* LBot *)
-/\ (!A S D. Gc S D ==> Gc (BAG_INSERT A S) D) (* Left Weakening *)
-/\ (!A S D. Gc S D ==> Gc S (BAG_INSERT A D)) (* Right Weakening *)
-/\ (!A S D. (Gc S D) /\ (S A >= 2)
-   ==> Gc (S - {|A|}) D) (* Left Contraction *)
-/\ (!A S D. (Gc S D) /\ (D A >= 2)
-   ==> Gc S (D - {|A|})) (* Right Contraction *)
-/\ (!A B S D. (Gc (BAG_INSERT A S) D) /\ (SING_BAG D \/ (D = EMPTY_BAG))
-   ==> (Gc (BAG_INSERT (A And B) S) D)) (* Left And 1 *)
-/\ (!A B S D. (Gc (BAG_INSERT B S) D) /\ (SING_BAG D \/ (D = EMPTY_BAG))
-   ==> (Gc (BAG_INSERT (A And B) S) D)) (* Left And 2 *)
-/\ (!A B S. (Gc S {|A|}) /\ (Gc S {|B|})
-   ==> (Gc S {|A And B|})) (* Right And *)
-/\ (!A B S D. (Gc (BAG_INSERT A S) D)
-    /\ (Gc (BAG_INSERT B S) D)
+/\ (Gi {|Bot|} {||})            (* LBot *)
+/\ (!A S D. Gi S D ==> Gi (BAG_INSERT A S) D) (* Left Weakening *)
+/\ (!A S D. Gi S D ==> Gi S (BAG_INSERT A D)) (* Right Weakening *)
+/\ (!A S D. (Gi S D) /\ (S A >= 2)
+   ==> Gi (S - {|A|}) D) (* Left Contraction *)
+/\ (!A S D. (Gi S D) /\ (D A >= 2)
+   ==> Gi S (D - {|A|})) (* Right Contraction *)
+/\ (!A B S D. (Gi (BAG_INSERT A S) D) /\ (SING_BAG D \/ (D = EMPTY_BAG))
+   ==> (Gi (BAG_INSERT (A And B) S) D)) (* Left And 1 *)
+/\ (!A B S D. (Gi (BAG_INSERT B S) D) /\ (SING_BAG D \/ (D = EMPTY_BAG))
+   ==> (Gi (BAG_INSERT (A And B) S) D)) (* Left And 2 *)
+/\ (!A B S. (Gi S {|A|}) /\ (Gi S {|B|})
+   ==> (Gi S {|A And B|})) (* Right And *)
+/\ (!A B S D. (Gi (BAG_INSERT A S) D)
+    /\ (Gi (BAG_INSERT B S) D)
     /\ (SING_BAG D \/ (D = EMPTY_BAG))
-   ==> (Gc (BAG_INSERT (A Or B) S) D) (* Left Or *)
-/\ (!A B S. (Gc S {|A|})
-   ==> (Gc S {|A Or B|})) (* Right Or 1 *)
-/\ (!A B S. (Gc S {|B|})
-   ==> (Gc S {|A Or B|})) (* Right Or 2 *)
-/\ (!A B S D. (Gc S {|A|} /\ (Gc (BAG_INSERT B S) D)
-               /\ (SING_BAG D \/ (D = EMPTY_BAG))
-   ==> (Gc (BAG_INSERT (A Imp B) S) D) (* Left Imp *)
-/\ (!A B S. (Gc (BAG_INSERT A S) {|B|})
-   ==> (Gc S {|A Imp B|})) (* Right Imp *)
-`;
+   ==> (Gi (BAG_INSERT (A Or B) S) D) (* Left Or *)
+/\ (!A B S. (Gi S {|A|})
+   ==> (Gi S {|A Or B|})) (* Right Or 1 *)
+/\ (!A B S. (Gi S {|B|})
+   ==> (Gi S {|A Or B|})) (* Right Or 2 *)
+/\ (!A B S D. (Gi S {|A|} /\ (Gi (BAG_INSERT B S) D)
+   /\ (SING_BAG D \/ (D = EMPTY_BAG))
+   ==> (Gi (BAG_INSERT (A Imp B) S) D) (* Left Imp *)
+/\ (!A B S. (Gi (BAG_INSERT A S) {|B|})
+   ==> (Gi S {|A Imp B|}))`; (* Right Imp *)
 
+               val GmThm = Define `GmThm A = Gm EMPTY_BAG {|A|}`
+
+(** Sequent Calculus (Gentzen System) for classical logic **)
+(* Gc is the 'deduciblility' relation for this system *)
 val (Gc_rules, Gc_induct, Gc_cases) = Hol_reln `
 (!A:'a formula. Gc {|A|} {|A|})            (* Ax *)
 /\ (Gc {|Bot|} {||})            (* LBot *)
@@ -167,5 +213,5 @@ val (Gc_rules, Gc_induct, Gc_cases) = Hol_reln `
 /\ (!A B S D. (Gc S (BAG_INSERT A D)) /\ (Gc (BAG_INSERT B S) D)
    ==> (Gc (BAG_INSERT (A Imp B) S) D)) (* Left Imp *)
 /\ (!A B S D. (Gc (BAG_INSERT A S) (BAG_INSERT B D))
-   ==> (Gc S (BAG_INSERT (A Imp B) D))) (* Right Imp *)
-`;
+   ==> (Gc S (BAG_INSERT (A Imp B) D)))`; (* Right Imp *)
+
